Proof (Trueif <--> \_ -> True)
* also (Falseif <--> \_ -> False)

thy/BDT.thy
@@ -11,10 +11,10 @@ fun ifex_var_set :: "'a ifex \<Rightarrow> 'a set" where
   "ifex_var_set Trueif = {}" |
   "ifex_var_set Falseif = {}"
 
-fun ifex_top_var_set :: "'a ifex \<Rightarrow> 'a set" where
-  "ifex_top_var_set (IF v t e) = {v}" |
-  "ifex_top_var_set Trueif = {}" |
-  "ifex_top_var_set Falseif = {}"
+fun ifex_top_var :: "'a ifex \<Rightarrow> 'a option" where
+  "ifex_top_var (IF v t e) = Some v" |
+  "ifex_top_var Trueif = None" |
+  "ifex_top_var Falseif = None"
 
 fun ifex_ordered :: "('a::linorder) ifex \<Rightarrow> bool" where
   "ifex_ordered (IF v t e) = ((\<forall>tv \<in> (ifex_var_set t \<union> ifex_var_set e). v < tv)
@@ -30,13 +30,56 @@ fun ifex_minimal :: "('a::linorder) ifex \<Rightarrow> bool" where
 definition ifex_bf2_rel where
   "ifex_bf2_rel = {(a,b). (\<forall>ass. a ass \<longleftrightarrow> val_ifex b ass) \<and> ifex_ordered b \<and> ifex_minimal b}"
 
-abbreviation ifex_robdt where
-  "ifex_robdt t \<equiv> ifex_ordered t \<and> ifex_minimal t"
+abbreviation ro_ifex where "ro_ifex t \<equiv> ifex_ordered t \<and> ifex_minimal t"
 
-lemma "ifex_robdt x \<Longrightarrow> ifex_robdt y \<Longrightarrow> \<forall>ass. val_ifex x ass = val_ifex y ass \<Longrightarrow> x = y"
-  oops
+lemma ifex_var_noinfluence: "x \<notin> ifex_var_set b \<Longrightarrow> val_ifex b (ass(x:=val)) = val_ifex b ass"
+  by (induction b, auto)
 
-lemma "single_valued ifex_bf2_rel"
-  oops
+lemma roifex_var_not_in_subtree:
+  assumes "ro_ifex b" and "b = IF v t e" 
+  shows "v \<notin> ifex_var_set t" and "v \<notin> ifex_var_set e"
+using assms by (induction, auto)
+
+lemma roifex_var_no_influence_subtree: 
+  assumes "ro_ifex b" and "b = IF v t e"
+  shows "val_ifex t (ass(v:=val)) = val_ifex t ass" 
+        "val_ifex e (ass(v:=val)) = val_ifex e ass"
+  using assms by (auto intro!: ifex_var_noinfluence dest: roifex_var_not_in_subtree)
+
+lemma roifex_set_var_subtree: 
+  assumes "ro_ifex b" and "b = IF v t e"
+  shows "val_ifex b (ass(v:=True)) = val_ifex t ass" 
+        "val_ifex b (ass(v:=False)) = val_ifex e ass"
+  using assms by (auto intro!: ifex_var_noinfluence dest: roifex_var_not_in_subtree)
+
+lemma roifex_Trueif_unique: "ro_ifex b \<Longrightarrow> \<forall>ass. val_ifex b ass \<Longrightarrow> b = Trueif"
+proof(induction b)
+  case (IF v b1 b2) with roifex_set_var_subtree[OF IF(3), of v b1 b2] show ?case by simp
+qed(auto)
+
+lemma roifex_Falseif_unique: "ro_ifex b \<Longrightarrow> \<forall>ass. \<not> val_ifex b ass \<Longrightarrow> b = Falseif"
+proof(induction b)
+  case (IF v b1 b2) with roifex_set_var_subtree[OF IF(3), of v b1 b2] show ?case by fastforce
+qed(auto)
+
+lemma "(f, b) \<in> ifex_bf2_rel \<Longrightarrow>  b = Trueif \<longleftrightarrow> f = (\<lambda>_. True)"
+  unfolding ifex_bf2_rel_def using roifex_Trueif_unique by auto
+
+lemma "(f, b) \<in> ifex_bf2_rel \<Longrightarrow>  b = Falseif \<longleftrightarrow> f = (\<lambda>_. False)"
+  unfolding ifex_bf2_rel_def using roifex_Falseif_unique by auto
+
+lemma "ro_ifex b \<Longrightarrow> x \<in> ifex_var_set b \<Longrightarrow>
+       \<exists>ass. val_ifex b (ass(x:=True)) \<noteq> val_ifex b (ass(x:=False))"
+oops
+
+lemma "ro_ifex x \<Longrightarrow> ro_ifex y \<Longrightarrow> \<forall>ass. val_ifex x ass = val_ifex y ass \<Longrightarrow> x = y"
+  proof(induction x arbitrary: y)
+  case (IF xv xb1 xb2) note IFinduction = IF thus ?case
+    proof(cases y)
+      case (IF yv yb1 yb2) 
+  thm IF IFinduction(3,4,5) IFinduction(1)[of yb1] IFinduction(2)[of yb2]
+  from IF IFinduction(5) have 0: "\<forall>ass. val_ifex (IF xv xb1 xb2) ass = val_ifex (IF yv yb1 yb2) ass"
+   by simp
+oops
 
 end
